## The Factor Theorem
$$
\displaylines{
\text{If } (x-a) \text{ is a factor of } f(x) \text{ then } f(-a) = 0 \\
f(x) \Longleftrightarrow f(a)=0 \\ \\
\text{If } (bx-a) \text{ is a factor of } f(x) \text{ then } f\left( \frac{a}{b} \right) = 0 \\
f(x) \Longleftrightarrow f\left( \frac{a}{b} \right)=0 \\ \\
\text{Show that } (2x-1) \text{ is a factor of } f(x)=2x^4-x^3+2x-1 \\
f\left( \frac{1}{2} \right)=2\left( \frac{1}{2} \right)^4-\left( \frac{1}{2} \right)^3+2\left( \frac{1}{2} \right)-1=0
}
$$
